trans.v
@@ -62,7 +62,7 @@ Fixpoint  trans_type (w1 l1: Syntax.term False) (tau : source.term) {struct tau}
                                                        let l := Syntax.var 0 in
                                                        let U := (ppair u l) in
                                                        arrow (subseq (ppair (shift 3 w1) l1) U)
- (*compm1_Type starts here*)                        (arrow (store U)
+ (*compm1_Type starts here*)                        (arrow (store u l)
                          (laters (exist nzero preworld ((* l1 = 3, u := 2, l:= 1, v = 0*)
                                           sigma nattp (*l1 = 4 u := 3, l := 2, v= 1, lv := 0*)
                                           (let u := Syntax.var 3 in
@@ -72,7 +72,7 @@ Fixpoint  trans_type (w1 l1: Syntax.term False) (tau : source.term) {struct tau}
                                               let U := ppair u l in
                                               let V := ppair v lv in
                                               (*u = 4, l = 3, subseq = 2, v = 1, lv = 0*)
-                                                    prod (prod (subseq U V) (store V))
+                                                    prod (prod (subseq U V) (store v lv))
                                                      (trans_type v lv tau'))))
                                     )
                        ))
